$\int_{- 3}^{3}{(x + 1)f(x)dx} = \int_{- 3}^{3}{\{ xf(x) + f(x)\}(x)dx} = \int_{- 3}^{3}{xf(x)dx} + \int_{- 3}^{3}{f(x)dx}$이다.

문제 조건에 의해 $\int_{- 3}^{ 3}{(x + 1)f(x) dx} = 36 + \int_{- 3}^{ 3}{f(x) dx}$이므로

$\int_{- 3}^{ 3}{xf(x) dx} + \int_{- 3}^{ 3}{f(x) dx} = 36 + \int_{- 3}^{ 3}{f(x) dx}$이다.

따라서 $\int_{- 3}^{ 3}{xf(x) dx} = 36$이다. ... ⑴

여기서 $f(x) = x^{2} + ax$이므로

$\int_{- 3}^{ 3}{xf(x) dx} = \int_{- 3}^{ 3}{x(x^{2} + ax) dx} = \int_{- 3}^{ 3}{(x^{3} + {ax}^{2}) dx}$이다.

적분 구간의 위끝과 아래끝의 부호는 다르고 절댓값은 같다.

따라서 기함수와 우함수의 적분 성질에 의해

$\int_{- 3}^{ 3}{(x^{3} + {ax}^{2}) dx} = \int_{- 3}^{ 3}{x^{3}dx} + \int_{- 3}^{ 3}{{ax}^{2}dx} = 0 + 2\int_{0}^{ 3}{{ax}^{2}dx}$이다. ... ⑵

⑴, ⑵에 의해 $2\int_{0}^{ 3}{{ax}^{2}dx} = 36$이다.

$2 \times \lbrack\frac{a}{3}x^{3}{\rbrack_{0}}^{3} = 18a = 36$에서 $a = 2$이다.
